

The KKT-conditions for \eqref{eq:system6} are as follows:
\begin{equation}
\label{KKT_system6}
\begin{aligned}
\bm{Dq} = \bm{B}^{T}\bm{\lambda}\\
\bm{I}^{T}_{\textrm{supp}}\bm{\lambda} = 0 \\
\bm{K} - \bm{P}\bm{\phi} - \bm{I}\bm{\gamma} + \bm{I}\bm{\xi} = 0 \\
\phi_j \geq 0  \text{ for } j = 1,...,m \\
\gamma_j \geq 0 \text{ for } j = 1,...,m \\
\xi_j \geq 0 \text{ for } j = 1,...,m \\
\phi_j(\rho_{j}l_{j}A_{j}-M) = 0 \text{ for } j = 1,...,m \\
\gamma_{j}(A_{j}-\overline{A_{j}}) = 0 \text{ for } j = 1,...,m \\
\xi_{j}(\underline{A_{j}}-A_{j}) = 0 \text{ for } j = 1,...,m \\
\end{aligned}
\end{equation}

\begin{align*}
&\bm{K} = \begin{bmatrix}
       -\frac{l_{1}q_{1}^2}{2E_{1}A_{1}^2}
       , -\frac{l_{2}q_{2}^2}{2E_{2}A_{2}}, \hdots,-\frac{l_{m}q_{m}^2}{2E_{m}A_{m}}
     \end{bmatrix}^T \\
&\bm{P} = \begin{bmatrix}
\rho_{1}l_{1} &  & \text{\large{0}}\\
 &  \ddots & & \\
\text{\large{0}} &  & \rho_{m}l_{m}
\end{bmatrix}\\
&\bm{I} = \begin{bmatrix}
1 &  &  \text{\large{0}}\\
  &  \ddots & \\
\text{\large{0}} &  & 1\\
\end{bmatrix}
\end{align*}

Computing the Hessian of our current objective function,
\begin{align*}
\bm{\bigtriangledown}^2 g(\bm{A},\bm{q},\bm{f}^{supp}) =
\left[\begin{array}{cc|cc|cc}
\frac{l_1q_1^2}{E_1A_1^3}&0& -\frac{l_1q_1}{E_1A_1^2} &0 & 0 & 0\\[0.3em]
0 &\ddots &0 & \ddots & 0 & \ddots\\[0.3em] \hline
-\frac{l_1q_1}{E_1A_1^2} & 0 & \frac{l_1}{E_1A_1} & 0 & 0 & 0\\[0.3em]
0 &\ddots & 0 &\ddots & 0 & \ddots\\[0.3em] \hline
0 & 0 & 0 & 0 & 0 & 0 \\[0.3em]
0 & \ddots & 0 & \ddots & 0 & \ddots\\[0.3em]
\end{array}\right],
\end{align*}
and letting $\bm{w}  \epsilon  \Omega$, we observe that

\begin{align*}
&\bm{w}^T\bm{\bigtriangledown}^2 g(\bm{A},\bm{q},\bm{f}^{supp})\bm{w} = \\
&\begin{bmatrix}
A_1 \hdots A_m & q_1 \hdots q_m & f_{1}^{supp} \hdots f_{m}^{supp}
\end{bmatrix}
\bm{\bigtriangledown}^2 g(\bm{A},\bm{q},\bm{f}^{supp})
\begin{bmatrix}
A_1 \\
\vdots\\
A_m\\
q_1\\
\vdots\\
q_m\\
f_{1}^{supp} \\
\vdots \\
f_{m}^ {supp}
\end{bmatrix} = 0.
\end{align*}
Thus $g(\bm{A},\bm{q},\bm{f}^{supp})$ is positive semi-definite, which is a sufficient condition for convexity. Since all our optimality constraints are affine, then according to \cite{KKT_suff}, (\ref{KKT_system6}) is both necessary and sufficient for optimality for \eqref{eq:system6}.

