
% DETTE ER UFERDIG
The KKT-conditions for \eqref{eq:system6} are as follows:
\begin{equation}
\label{KKT_system7}
\begin{aligned}
\bm{Dq} = \bm{B}^{T}\bm{\lambda}\\
\bm{I}^{T}_{\textrm{supp}}\bm{\lambda} = 0 \\
\bm{K} + \frac{\mu}{M-\sum\limits_{j=1}^m\rho_{j}l_{j}A_{j}}\bm{T} - \mu\bm{C} = 0 \\
\bm{Bq} - \bm{I}_{\textrm{supp}}\bm{f}^{\textrm{supp}} - \bm{I}_{\textrm{ext}}\bm{f}^{\textrm{ext}} = 0 \\
(\bm{Bq} - \bm{I}_{\textrm{supp}}\bm{f}^{\textrm{supp}} - \bm{I}_{\textrm{ext}}\bm{f}^{\textrm{ext}})^T\bm{\lambda} = 0 \\
\bm{K} + \bm{T}\bm{\phi} + \bm{\gamma} - \bm{\xi} = 0 \\
\phi_j \geq 0  \text{ for } j = 1,...,m \\
\gamma_j \geq 0 \text{ for } j = 1,...,m \\
\xi_j \geq 0 \text{ for } j = 1,...,m \\
\phi_j(M-\sum\limits_{j=1}^m\rho_{j}l_{j}A_{j}) = 0 \text{ for } j = 1,...,m \\
\gamma_{j}(A_{j}-\overline{A_{j}}) = 0 \text{ for } j = 1,...,m \\
\xi_{j}(\underline{A_{j}}-A_{j}) = 0 \text{ for } j = 1,...,m \\
\end{aligned}
\end{equation}

\begin{align*}
&\bm{T} = \begin{bmatrix}
       \rho_{1}l_{1}
       , \hdots,\rho_{m}l_{m}
     \end{bmatrix}^T \\
&\bm{C} = \begin{bmatrix}
\frac{1}{A_1-\underline{A_{1}}} - \frac{1}{\overline{A_{1}}-A_{1}}, \hdots, \frac{1}{A_m-\underline{A_{m}}} - \frac{1}{\overline{A_{m}}-A_{m}}
\end{bmatrix}^T
\end{align*}
By comparing the two systems, we see that the approximations to the Lagrange multipliers corresponding to the inequality constraints in (\ref{KKT_system6}), in terms of an optimum for (\ref{KKT_system7}), must satisfy the following:

\begin{align*}
\frac{\mu}{M-\sum\limits_{j=1}^m\rho_jl_jA_j}
\begin{bmatrix}
\rho_1l_1 \\
\vdots \\
\rho_ml_m\\
\end{bmatrix} &= 
\begin{bmatrix}
\rho_1l_1 & & \text{\large{0}} \\[0.5em]
 & \ddots &  \\
\text{\large{0}} & & \rho_ml_m \\[0.5em]
\end{bmatrix}
\begin{bmatrix}
\phi_1 \\
\vdots \\
\phi_m\\
\end{bmatrix}\\
\begin{bmatrix}
\gamma_1 \\
\vdots \\
\gamma_m\\
\end{bmatrix} &= \mu
\begin{bmatrix}
\frac{1}{\overline{A}_1-A_1} \\
\vdots \\
\frac{1}{\overline{A}_m-A_m}\\
\end{bmatrix}\\
\begin{bmatrix}
\xi_1 \\
\vdots \\
\xi_m\\
\end{bmatrix} 
&= \mu
\begin{bmatrix}
\frac{1}{A_1-\underline{A}_1} \\
\vdots \\
\frac{1}{A_m-\underline{A}_m}
\end{bmatrix}.
\end{align*}
From this we conclude that
\begin{align*}
\phi_j = \frac{\mu}{M-\sum\limits_{j=1}^m\rho_jl_jA_j} \text{ for } j = 1,..,m \\
\gamma_j = \frac{1}{\overline{A}_j-A_j} \text{ for } j = 1,..,m \\
\xi_j = \frac{1}{A_j-\underline{A}_j} \text{ for } j = 1,..,m.
\end{align*}